work on ptr mono1

proof/ptr.v
@@ -8,37 +8,87 @@ Section ptr.
 
 Context (layout: Layout).
 
-Definition align :=
+Notation align := (
   match layout with
   | mkLayout align size => align
-  end.
+  end).
 
-Definition size :=
+Notation size := (
   match layout with
   | mkLayout align size => size
-  end.
+  end).
 
 Context (ptr_ty: PtrTy).
 
 Notation t := (TPtr ptr_ty layout).
 
-Definition Constraints addr align :=
+Notation Constraints addr align := (
   match ptr_ty with
   | Raw => true
   | Ref => ((addr >? 0)%Z && (addr mod (Z.of_nat align) =? 0)%Z)%bool
-  end = true.
+  end).
 
 Inductive ValidPtr : Value -> Type :=
-  | mkValidPtr addr p : Constraints addr align -> ValidPtr (VPtr addr p).
+  | mkValidPtr addr p : Constraints addr align = true -> ValidPtr (VPtr addr p).
 
 Lemma valid_ptr (v: Value) (H: is_valid_for t v) :
   ValidPtr v.
 Proof.
+
 unfold is_valid_for in H.
 Admitted.
 
 Lemma ptr_mono1 : mono1 t.
 Proof.
+intros Hwf v1 v2 Hle Hv1 Hv2.
+assert (exists a b, VPtr a b = v1). {
+  destruct Hv1. unfold decode,decode_ptr in H.
+  destruct (unwrap_abstract x); cycle 1. { discriminate H. }
+  simpl in H.
+  destruct (decode_int_raw PTR_SIZE Unsigned l); cycle 1. { discriminate H. }
+  simpl in H.
+  unfold utils.assuming in H. simpl in H.
+  destruct (Constraints i align) eqn:E; cycle 1. { discriminate H. }
+  simpl in H.
+  injection H.
+  intros L.
+  (* TODO better solution? *)
+  exists i. exists ((ssrfun.Option.bind
+          (utils.assuming_const
+             (forallb
+                (fun x0 : AbstractByte =>
+                 match x0 with
+                 | Uninit => false
+                 | Init _ (Some a) =>
+                     match
+                       match x with
+                       | Init _ p0 :: _ => p0
+                       | _ => None
+                       end
+                     with
+                     | Some b0 => P_EQ a b0
+                     | None => false
+                     end
+                 | Init _ None =>
+                     match
+                       match x with
+                       | Init _ p0 :: _ => p0
+                       | _ => None
+                       end
+                     with
+                     | Some _ => false
+                     | None => true
+                     end
+                 end) x))
+          match x with
+          | Init _ p :: _ => p
+          | _ => None
+          end)). auto.
+}
+destruct H as [addr].
+destruct H as [p Hv].
+rewrite <- Hv.
+rewrite <- Hv in Hle.
 Admitted.
 
 Lemma ptr_mono2 : mono2 t.
